theories/modules/LModTr.v
@@ -3,32 +3,32 @@ Require Import Common.
 Module LModTr.
   Definition pure_state {S E} : E ~> stateT S (itree E) := λ _ e s, x <- trigger e;; Ret (s, x).
 
-  Definition handle_stateE {E} : stateE ~> stateT Any.t (itree E) :=
+  Definition handle_stateE {E} : lstateE ~> stateT lstateT (itree E) :=
     λ _ e glob,
       match e with
       | SUpdate run => Ret (run glob)
       end.
 
-  Definition interp_stateE {E} : itree (stateE +' E) ~> stateT Any.t (itree E) :=
+  Definition interp_stateE {E} : itree (lstateE +' E) ~> stateT lstateT (itree E) :=
     State.interp_state (case_ handle_stateE pure_state).
 
   Definition ths_state : Type := nat * list (itree lmodE Any.t).
 
   Definition handle_callE (prog: string → option (Any.t → itree lmodE Any.t))
-      : ths_state → itreeV (stateE +' coreE) (ths_state + Any.t) :=
+      : ths_state → itreeV (lstateE +' coreE) (ths_state + Any.t) :=
     λ '(tid, ths),
       match base.lookup tid ths with
-      | None => inl (triggerUB)
+      | None => itreeV_nvis (triggerUB)
       | Some itr =>
           match observe (itr: itree lmodE Any.t) with
           | RetF rv =>
-              inl (if Nat.eq_dec tid 0 then Ret (inr rv) else triggerUB)
+              itreeV_nvis (if Nat.eq_dec tid 0 then Ret (inr rv) else triggerUB)
           | TauF itr' =>
-              inl (Ret (inl (tid, <[tid := itr']> ths)))
+              itreeV_nvis (Ret (inl (tid, <[tid := itr']> ths)))
           | VisF (inr1 e) k =>
-              inr (existT _ (subevent _ e, λ v, Ret (inl (tid, <[tid := k v]> ths))))
+              itreeV_vis (subevent _ e) (λ v, Ret (inl (tid, <[tid := k v]> ths)))
           | VisF (inl1 e) k =>
-              inl
+              itreeV_nvis
                 (match e in callE T return (T → _) → _ with
                  | Call fn arg =>
                     λ k,
@@ -46,9 +46,9 @@ Module LModTr.
           end
       end.
 
-  Definition interp_callE prog (itr : itree lmodE Any.t) : itree (stateE +' coreE) Any.t :=
+  Definition interp_callE prog (itr : itree lmodE Any.t) : itree (lstateE +' coreE) Any.t :=
     iterV (handle_callE prog) (0, [itr]).
 
-  Definition trans prog (itr : itree lmodE Any.t) (st : Any.t): itree coreE _ :=
+  Definition trans prog (itr : itree lmodE Any.t) (st : lstateT): itree coreE _ :=
     interp_stateE Any.t (interp_callE prog itr) st.
 End LModTr.
