theories/simulations/gsim/GSimAux.v
@@ -33,32 +33,32 @@ Section props.
   Lemma gsim_flag r g RR p_s p_t p_s1 p_t1 i_s i_t :
     smj_le p_s1 p_s →
     smj_le p_t1 p_t →
-    gpaco7 _gsim (cpn7 _gsim) r g (Any.t * Any.t)%type (Any.t * Any.t)%type RR p_s1 p_t1
+    gpaco7 _gsim (cpn7 _gsim) r g (lstateT * Any.t)%type (lstateT * Any.t)%type RR p_s1 p_t1
       i_s i_t →
-    gpaco7 _gsim (cpn7 _gsim) r g (Any.t * Any.t)%type (Any.t * Any.t)%type RR p_s p_t
+    gpaco7 _gsim (cpn7 _gsim) r g (lstateT * Any.t)%type (lstateT * Any.t)%type RR p_s p_t
       i_s i_t.
   Proof using. guclo flagC_spec; econs; eauto. Qed.
 
   Lemma gsim_tau_src r g RR p_s p_t st_s itr_t prog_s tid_s tp_s k :
     tp_s !! tid_s = Some (⇓cris (tau;; k)) →
-    gpaco7 _gsim (cpn7 _gsim) r g (Any.t * Any.t)%type (Any.t * Any.t)%type RR smj_top p_t
+    gpaco7 _gsim (cpn7 _gsim) r g (lstateT * Any.t)%type (lstateT * Any.t)%type RR smj_top p_t
       (LModTr.interp_stateE Any.t
         (iterV (LModTr.handle_callE prog_s)
           (tid_s, <[tid_s := (⇓cris k)]> tp_s)) st_s)
       itr_t →
-    gpaco7 _gsim (cpn7 _gsim) r g (Any.t * Any.t)%type (Any.t * Any.t)%type RR p_s p_t
+    gpaco7 _gsim (cpn7 _gsim) r g (lstateT * Any.t)%type (lstateT * Any.t)%type RR p_s p_t
       (LModTr.interp_stateE Any.t (iterV (LModTr.handle_callE prog_s) (tid_s, tp_s)) st_s)
       itr_t.
   Proof using. intros Hi ?. giter_s. s. rewrite Hi; ss. gstep_s. gcNormS. done. Qed.
 
   Lemma gsim_tau_tgt r g RR p_s p_t itr_s st_t prog_t tid_t tp_t k :
     tp_t !! tid_t = Some (⇓cris (tau;; k)) →
-    gpaco7 _gsim (cpn7 _gsim) r g (Any.t * Any.t)%type (Any.t * Any.t)%type RR p_s smj_top
+    gpaco7 _gsim (cpn7 _gsim) r g (lstateT * Any.t)%type (lstateT * Any.t)%type RR p_s smj_top
       itr_s
       (LModTr.interp_stateE Any.t
         (iterV (LModTr.handle_callE prog_t)
           (tid_t, <[tid_t := ⇓cris k]> tp_t)) st_t) →
-    gpaco7 _gsim (cpn7 _gsim) r g (Any.t * Any.t)%type (Any.t * Any.t)%type RR p_s p_t
+    gpaco7 _gsim (cpn7 _gsim) r g (lstateT * Any.t)%type (lstateT * Any.t)%type RR p_s p_t
       itr_s
       (LModTr.interp_stateE Any.t (iterV (LModTr.handle_callE prog_t) (tid_t, tp_t)) st_t).
   Proof using. intros Hi ?. giter_t; rewrite /= Hi; ss. gstep_t; gcNormT. done. Qed.
@@ -66,12 +66,12 @@ Section props.
   Lemma gsim_Choose_src r g RR p_s p_t st_s prog_s tid_s tp_s X k itr_t :
     tp_s !! tid_s = Some (⇓cris (x <- trigger (Choose X);; k x)) →
     (∃ (x : X),
-      gpaco7 _gsim (cpn7 _gsim) r g (Any.t * Any.t)%type (Any.t * Any.t)%type RR smj_top p_t
+      gpaco7 _gsim (cpn7 _gsim) r g (lstateT * Any.t)%type (lstateT * Any.t)%type RR smj_top p_t
         (LModTr.interp_stateE Any.t
           (iterV (LModTr.handle_callE prog_s)
             (tid_s, <[tid_s := ⇓cris (k x)]> tp_s)) st_s)
         itr_t) →
-    gpaco7 _gsim (cpn7 _gsim) r g (Any.t * Any.t)%type (Any.t * Any.t)%type RR p_s p_t
+    gpaco7 _gsim (cpn7 _gsim) r g (lstateT * Any.t)%type (lstateT * Any.t)%type RR p_s p_t
       (LModTr.interp_stateE Any.t (iterV (LModTr.handle_callE prog_s) (tid_s, tp_s)) st_s)
       itr_t.
   Proof using.
@@ -82,12 +82,12 @@ Section props.
   Lemma gsim_Choose_tgt r g RR p_s p_t st_t prog_t tid_t tp_t X k itr_s :
     tp_t !! tid_t = Some (⇓cris (x <- trigger (Choose X);; k x)) →
     (∀ (x : X),
-      gpaco7 _gsim (cpn7 _gsim) r g (Any.t * Any.t)%type (Any.t * Any.t)%type RR p_s smj_top
+      gpaco7 _gsim (cpn7 _gsim) r g (lstateT * Any.t)%type (lstateT * Any.t)%type RR p_s smj_top
         itr_s
         (LModTr.interp_stateE Any.t
           (iterV (LModTr.handle_callE prog_t)
             (tid_t, <[tid_t := ⇓cris (k x)]> tp_t)) st_t)) →
-    gpaco7 _gsim (cpn7 _gsim) r g (Any.t * Any.t)%type (Any.t * Any.t)%type RR p_s p_t
+    gpaco7 _gsim (cpn7 _gsim) r g (lstateT * Any.t)%type (lstateT * Any.t)%type RR p_s p_t
       itr_s
       (LModTr.interp_stateE Any.t (iterV (LModTr.handle_callE prog_t) (tid_t, tp_t)) st_t).
   Proof using.
@@ -98,12 +98,12 @@ Section props.
   Lemma gsim_Take_src r g RR p_s p_t st_s prog_s tid_s tp_s X k itr_t :
     tp_s !! tid_s = Some (⇓cris (x <- trigger (Take X);; k x)) →
     (∀ (x : X),
-      gpaco7 _gsim (cpn7 _gsim) r g (Any.t * Any.t)%type (Any.t * Any.t)%type RR smj_top p_t
+      gpaco7 _gsim (cpn7 _gsim) r g (lstateT * Any.t)%type (lstateT * Any.t)%type RR smj_top p_t
         (LModTr.interp_stateE Any.t
           (iterV (LModTr.handle_callE prog_s)
             (tid_s, <[tid_s := ⇓cris (k x)]> tp_s)) st_s)
         itr_t) →
-    gpaco7 _gsim (cpn7 _gsim) r g (Any.t * Any.t)%type (Any.t * Any.t)%type RR p_s p_t
+    gpaco7 _gsim (cpn7 _gsim) r g (lstateT * Any.t)%type (lstateT * Any.t)%type RR p_s p_t
       (LModTr.interp_stateE Any.t (iterV (LModTr.handle_callE prog_s) (tid_s, tp_s)) st_s)
       itr_t.
   Proof using.
@@ -114,12 +114,12 @@ Section props.
   Lemma gsim_Take_tgt r g RR p_s p_t st_t prog_t tid_t tp_t X k itr_s :
     tp_t !! tid_t = Some (⇓cris (x <- trigger (Take X);; k x)) →
     (∃ (x : X),
-      gpaco7 _gsim (cpn7 _gsim) r g (Any.t * Any.t)%type (Any.t * Any.t)%type RR p_s smj_top
+      gpaco7 _gsim (cpn7 _gsim) r g (lstateT * Any.t)%type (lstateT * Any.t)%type RR p_s smj_top
         itr_s
         (LModTr.interp_stateE Any.t
           (iterV (LModTr.handle_callE prog_t)
             (tid_t, <[tid_t := ⇓cris (k x)]> tp_t)) st_t)) →
-    gpaco7 _gsim (cpn7 _gsim) r g (Any.t * Any.t)%type (Any.t * Any.t)%type RR p_s p_t
+    gpaco7 _gsim (cpn7 _gsim) r g (lstateT * Any.t)%type (lstateT * Any.t)%type RR p_s p_t
       itr_s
       (LModTr.interp_stateE Any.t (iterV (LModTr.handle_callE prog_t) (tid_t, tp_t)) st_t).
   Proof using.
@@ -132,14 +132,14 @@ Section props.
     tp_s !! tid_s = Some (⇓cris (x <- trigger (IO fn args);; k_s x)) →
     tp_t !! tid_t = Some (⇓cris (x <- trigger (IO fn args);; k_t x)) →
     (∀ (ret : O),
-      gpaco7 _gsim (cpn7 _gsim) r g (Any.t * Any.t)%type (Any.t * Any.t)%type RR smj_top smj_top
+      gpaco7 _gsim (cpn7 _gsim) r g (lstateT * Any.t)%type (lstateT * Any.t)%type RR smj_top smj_top
         (LModTr.interp_stateE Any.t
           (iterV (LModTr.handle_callE prog_s)
             (tid_s, <[tid_s := ⇓cris (k_s ret)]> tp_s)) st_s)
         (LModTr.interp_stateE Any.t
           (iterV (LModTr.handle_callE prog_t)
             (tid_t, <[tid_t := ⇓cris (k_t ret)]> tp_t)) st_t)) →
-    gpaco7 _gsim (cpn7 _gsim) r g (Any.t * Any.t)%type (Any.t * Any.t)%type RR p_s p_t
+    gpaco7 _gsim (cpn7 _gsim) r g (lstateT * Any.t)%type (lstateT * Any.t)%type RR p_s p_t
       (LModTr.interp_stateE Any.t (iterV (LModTr.handle_callE prog_s) (tid_s, tp_s)) st_s)
       (LModTr.interp_stateE Any.t (iterV (LModTr.handle_callE prog_t) (tid_t, tp_t)) st_t).
   Proof using.
@@ -151,12 +151,12 @@ Section props.
 
   Lemma gsim_Call_src r g RR p_s p_t st_s st_t prog_s prog_t tid_s tid_t tp_s tp_t fn args k :
     tp_s !! tid_s = Some (⇓cris (x <- trigger (Call fn args);; k x)) →
-    (gpaco7 _gsim (cpn7 _gsim) r g (Any.t * Any.t)%type (Any.t * Any.t)%type RR smj_top p_t
+    (gpaco7 _gsim (cpn7 _gsim) r g (lstateT * Any.t)%type (lstateT * Any.t)%type RR smj_top p_t
       (LModTr.interp_stateE Any.t
         (iterV (LModTr.handle_callE prog_s)
           (tid_s, <[tid_s := bd <- (prog_s fn)?;; x <- (bd args);; ⇓cris (tau;; k x)]> tp_s)) st_s)
       (LModTr.interp_stateE Any.t (iterV (LModTr.handle_callE prog_t) (tid_t, tp_t)) st_t)) →
-    gpaco7 _gsim (cpn7 _gsim) r g (Any.t * Any.t)%type (Any.t * Any.t)%type RR p_s p_t
+    gpaco7 _gsim (cpn7 _gsim) r g (lstateT * Any.t)%type (lstateT * Any.t)%type RR p_s p_t
       (LModTr.interp_stateE Any.t (iterV (LModTr.handle_callE prog_s) (tid_s, tp_s)) st_s)
       (LModTr.interp_stateE Any.t (iterV (LModTr.handle_callE prog_t) (tid_t, tp_t)) st_t).
   Proof using.
@@ -172,12 +172,12 @@ Section props.
 
   Lemma gsim_Call_tgt r g RR p_s p_t st_s st_t prog_s prog_t tid_s tid_t tp_s tp_t fn args k :
     tp_t !! tid_t = Some (⇓cris (x <- trigger (Call fn args);; k x)) →
-    (gpaco7 _gsim (cpn7 _gsim) r g (Any.t * Any.t)%type (Any.t * Any.t)%type RR p_s smj_top
+    (gpaco7 _gsim (cpn7 _gsim) r g (lstateT * Any.t)%type (lstateT * Any.t)%type RR p_s smj_top
       (LModTr.interp_stateE Any.t (iterV (LModTr.handle_callE prog_s) (tid_s, tp_s)) st_s)
       (LModTr.interp_stateE Any.t
         (iterV (LModTr.handle_callE prog_t)
           (tid_t, <[tid_t := bd <- (prog_t fn)?;; x <- (bd args);; ⇓cris (tau;; k x)]> tp_t)) st_t)) →
-    gpaco7 _gsim (cpn7 _gsim) r g (Any.t * Any.t)%type (Any.t * Any.t)%type RR p_s p_t
+    gpaco7 _gsim (cpn7 _gsim) r g (lstateT * Any.t)%type (lstateT * Any.t)%type RR p_s p_t
       (LModTr.interp_stateE Any.t (iterV (LModTr.handle_callE prog_s) (tid_s, tp_s)) st_s)
       (LModTr.interp_stateE Any.t (iterV (LModTr.handle_callE prog_t) (tid_t, tp_t)) st_t).
   Proof using.
@@ -193,13 +193,13 @@ Section props.
 
   Lemma gsim_Spawn_src r g RR p_s p_t itr_t st_s prog_s tid_s tp_s fn args k :
     tp_s !! tid_s = Some (⇓cris (x <- trigger (Spawn fn args);; k x)) →
-    (gpaco7 _gsim (cpn7 _gsim) r g (Any.t * Any.t)%type (Any.t * Any.t)%type RR smj_top p_t
+    (gpaco7 _gsim (cpn7 _gsim) r g (lstateT * Any.t)%type (lstateT * Any.t)%type RR smj_top p_t
       (LModTr.interp_stateE Any.t
         (bd <- (prog_s fn)?;;
         iterV (LModTr.handle_callE prog_s)
           (tid_s, <[tid_s := ⇓cris (k (List.length tp_s))]> tp_s ++ [bd args])) st_s)
       itr_t) →
-    gpaco7 _gsim (cpn7 _gsim) r g (Any.t * Any.t)%type (Any.t * Any.t)%type RR p_s p_t
+    gpaco7 _gsim (cpn7 _gsim) r g (lstateT * Any.t)%type (lstateT * Any.t)%type RR p_s p_t
       (LModTr.interp_stateE Any.t (iterV (LModTr.handle_callE prog_s) (tid_s, tp_s)) st_s)
       itr_t.
   Proof using.
@@ -211,13 +211,13 @@ Section props.
 
   Lemma gsim_Spawn_tgt r g RR p_s p_t itr_s st_t prog_t tid_t tp_t fn args k :
     tp_t !! tid_t = Some (⇓cris (x <- trigger (Spawn fn args);; k x)) →
-    (gpaco7 _gsim (cpn7 _gsim) r g (Any.t * Any.t)%type (Any.t * Any.t)%type RR p_s smj_top
+    (gpaco7 _gsim (cpn7 _gsim) r g (lstateT * Any.t)%type (lstateT * Any.t)%type RR p_s smj_top
       (itr_s)
       (LModTr.interp_stateE Any.t
         (bd <- (prog_t fn)?;;
         iterV (LModTr.handle_callE prog_t)
           (tid_t, <[tid_t := ⇓cris (k (List.length tp_t))]> tp_t ++ [bd args])) st_t)) →
-    gpaco7 _gsim (cpn7 _gsim) r g (Any.t * Any.t)%type (Any.t * Any.t)%type RR p_s p_t
+    gpaco7 _gsim (cpn7 _gsim) r g (lstateT * Any.t)%type (lstateT * Any.t)%type RR p_s p_t
       (itr_s)
       (LModTr.interp_stateE Any.t (iterV (LModTr.handle_callE prog_t) (tid_t, tp_t)) st_t).
   Proof using.
@@ -229,48 +229,48 @@ Section props.
 
   Lemma gsim_GetTid_src r g RR p_s p_t itr_t st_s prog_s tid_s tp_s k :
     tp_s !! tid_s = Some (⇓cris (x <- trigger GetTid;; k x)) →
-    (gpaco7 _gsim (cpn7 _gsim) r g (Any.t * Any.t)%type (Any.t * Any.t)%type RR smj_top p_t
+    (gpaco7 _gsim (cpn7 _gsim) r g (lstateT * Any.t)%type (lstateT * Any.t)%type RR smj_top p_t
       (LModTr.interp_stateE Any.t
         (iterV (LModTr.handle_callE prog_s)
           (tid_s, <[tid_s := ⇓cris (k (tid_s))]> tp_s)) st_s)
       itr_t) →
-    gpaco7 _gsim (cpn7 _gsim) r g (Any.t * Any.t)%type (Any.t * Any.t)%type RR p_s p_t
+    gpaco7 _gsim (cpn7 _gsim) r g (lstateT * Any.t)%type (lstateT * Any.t)%type RR p_s p_t
       (LModTr.interp_stateE Any.t (iterV (LModTr.handle_callE prog_s) (tid_s, tp_s)) st_s)
       itr_t.
   Proof using. intros Hi Hk. giter_s. rewrite /= Hi; ss. gstep_s. by ired. Qed.
 
   Lemma gsim_GetTid_tgt r g RR p_s p_t itr_s st_t prog_t tid_t tp_t k :
     tp_t !! tid_t = Some (⇓cris (x <- trigger GetTid;; k x)) →
-    (gpaco7 _gsim (cpn7 _gsim) r g (Any.t * Any.t)%type (Any.t * Any.t)%type RR p_s smj_top
+    (gpaco7 _gsim (cpn7 _gsim) r g (lstateT * Any.t)%type (lstateT * Any.t)%type RR p_s smj_top
       (itr_s)
       (LModTr.interp_stateE Any.t
         (iterV (LModTr.handle_callE prog_t)
           (tid_t, <[tid_t := ⇓cris (k (tid_t))]> tp_t)) st_t)) →
-    gpaco7 _gsim (cpn7 _gsim) r g (Any.t * Any.t)%type (Any.t * Any.t)%type RR p_s p_t
+    gpaco7 _gsim (cpn7 _gsim) r g (lstateT * Any.t)%type (lstateT * Any.t)%type RR p_s p_t
       (itr_s)
       (LModTr.interp_stateE Any.t (iterV (LModTr.handle_callE prog_t) (tid_t, tp_t)) st_t).
   Proof using. intros Hi Hk. giter_t. rewrite /= Hi; ss. gstep_t. by ired. Qed.
 
   Lemma gsim_Yield_src r g RR p_s p_t itr_t st_s prog_s tid_s tid_s2 tp_s k :
     tp_s !! tid_s = Some (⇓cris (x <- trigger (Yield tid_s2);; k x)) →
-    (gpaco7 _gsim (cpn7 _gsim) r g (Any.t * Any.t)%type (Any.t * Any.t)%type RR smj_top p_t
+    (gpaco7 _gsim (cpn7 _gsim) r g (lstateT * Any.t)%type (lstateT * Any.t)%type RR smj_top p_t
       (LModTr.interp_stateE Any.t
         (iterV (LModTr.handle_callE prog_s)
           (tid_s2, <[tid_s := ⇓cris (k ())]> tp_s)) st_s)
       itr_t) →
-    gpaco7 _gsim (cpn7 _gsim) r g (Any.t * Any.t)%type (Any.t * Any.t)%type RR p_s p_t
+    gpaco7 _gsim (cpn7 _gsim) r g (lstateT * Any.t)%type (lstateT * Any.t)%type RR p_s p_t
       (LModTr.interp_stateE Any.t (iterV (LModTr.handle_callE prog_s) (tid_s, tp_s)) st_s)
       itr_t.
   Proof using. intros Hi Hk. giter_s. rewrite /= Hi; ss. gstep_s. by ired. Qed.
 
   Lemma gsim_Yield_tgt r g RR p_s p_t itr_s st_t prog_t tid_t tid_t2 tp_t k :
     tp_t !! tid_t = Some (⇓cris (x <- trigger (Yield tid_t2);; k x)) →
-    (gpaco7 _gsim (cpn7 _gsim) r g (Any.t * Any.t)%type (Any.t * Any.t)%type RR p_s smj_top
+    (gpaco7 _gsim (cpn7 _gsim) r g (lstateT * Any.t)%type (lstateT * Any.t)%type RR p_s smj_top
       (itr_s)
       (LModTr.interp_stateE Any.t
         (iterV (LModTr.handle_callE prog_t)
           (tid_t2, <[tid_t := ⇓cris (k ())]> tp_t)) st_t)) →
-    gpaco7 _gsim (cpn7 _gsim) r g (Any.t * Any.t)%type (Any.t * Any.t)%type RR p_s p_t
+    gpaco7 _gsim (cpn7 _gsim) r g (lstateT * Any.t)%type (lstateT * Any.t)%type RR p_s p_t
       (itr_s)
       (LModTr.interp_stateE Any.t (iterV (LModTr.handle_callE prog_t) (tid_t, tp_t)) st_t).
   Proof using. intros Hi Hk. giter_t. rewrite /= Hi; ss. gstep_t. by ired. Qed.
@@ -278,58 +278,55 @@ Section props.
   Lemma gsim_SGet_tgt r g RR p_s p_t itr_s st_t prog_t tid_t tp_t key k r_t :
     tp_t !! tid_t = Some (⇓cris (x <- trigger (SGet key);; k x)) →
     map_Forall (const is_Some) st_t →
-    (gpaco7 _gsim (cpn7 _gsim) r g (Any.t * Any.t)%type (Any.t * Any.t)%type RR p_s smj_top
+    (gpaco7 _gsim (cpn7 _gsim) r g (lstateT * Any.t)%type (lstateT * Any.t)%type RR p_s smj_top
       itr_s
       (LModTr.interp_stateE Any.t
         (iterV (LModTr.handle_callE prog_t)
           (tid_t, <[tid_t := ⇓cris (k (default ()↑ (mjoin (st_t !! key))))]> tp_t))
-        (Any.pair (ModTr.state_encode st_t) r_t))) →
-    gpaco7 _gsim (cpn7 _gsim) r g (Any.t * Any.t)%type (Any.t * Any.t)%type RR p_s p_t
+        (st_t, r_t))) →
+    gpaco7 _gsim (cpn7 _gsim) r g (lstateT * Any.t)%type (lstateT * Any.t)%type RR p_s p_t
       itr_s
       (LModTr.interp_stateE Any.t (iterV (LModTr.handle_callE prog_t) (tid_t, tp_t))
-        (Any.pair (ModTr.state_encode st_t) r_t)).
+        (st_t, r_t)).
   Proof using.
     intros Hin ? ?.
-    giter_t; rewrite /= Hin; ss. gsteps_t. cSimpl. ired.
-    rewrite ModTr.state_encode_decode //.
+    giter_t; rewrite /= Hin; ss. gsteps_t. cSimpl. ired. eauto.
   Qed.
 
   Lemma gsim_SGet_src r g RR p_s p_t itr_t st_s prog_s tid_s tp_s key k r_s :
     tp_s !! tid_s = Some (⇓cris (x <- trigger (SGet key);; k x)) →
     map_Forall (const is_Some) st_s →
-    (gpaco7 _gsim (cpn7 _gsim) r g (Any.t * Any.t)%type (Any.t * Any.t)%type RR smj_top p_t
+    (gpaco7 _gsim (cpn7 _gsim) r g (lstateT * Any.t)%type (lstateT * Any.t)%type RR smj_top p_t
       (LModTr.interp_stateE Any.t
         (iterV (LModTr.handle_callE prog_s)
           (tid_s, <[tid_s := ⇓cris (k (default ()↑ (mjoin (st_s !! key))))]> tp_s))
-        (Any.pair (ModTr.state_encode st_s) r_s))
+        (st_s, r_s))
       itr_t) →
-    gpaco7 _gsim (cpn7 _gsim) r g (Any.t * Any.t)%type (Any.t * Any.t)%type RR p_s p_t
+    gpaco7 _gsim (cpn7 _gsim) r g (lstateT * Any.t)%type (lstateT * Any.t)%type RR p_s p_t
       (LModTr.interp_stateE Any.t (iterV (LModTr.handle_callE prog_s) (tid_s, tp_s))
-        (Any.pair (ModTr.state_encode st_s) r_s))
+        (st_s, r_s))
       itr_t.
   Proof using.
     intros Hin ? ?.
-    giter_s; rewrite /= Hin; ss. gsteps_s. cSimpl. ired.
-    rewrite ModTr.state_encode_decode //.
+    giter_s; rewrite /= Hin; ss. gsteps_s. cSimpl. ired. eauto.
   Qed.
 
   Lemma gsim_SPut_tgt r g RR p_s p_t itr_s st_t prog_t tid_t tp_t key val k r_t :
     tp_t !! tid_t = Some (⇓cris (x <- trigger (SPut key val);; k x)) →
     map_Forall (const is_Some) st_t →
-    (gpaco7 _gsim (cpn7 _gsim) r g (Any.t * Any.t)%type (Any.t * Any.t)%type RR p_s smj_top
+    (gpaco7 _gsim (cpn7 _gsim) r g (lstateT * Any.t)%type (lstateT * Any.t)%type RR p_s smj_top
       itr_s
       (LModTr.interp_stateE Any.t
         (iterV (LModTr.handle_callE prog_t)
           (tid_t, <[tid_t := ⇓cris (k ())]> tp_t))
-        (Any.pair (ModTr.state_encode (<[key := Some val]> st_t)) r_t))) →
-    gpaco7 _gsim (cpn7 _gsim) r g (Any.t * Any.t)%type (Any.t * Any.t)%type RR p_s p_t
+        (<[key := Some val]> st_t, r_t))) →
+    gpaco7 _gsim (cpn7 _gsim) r g (lstateT * Any.t)%type (lstateT * Any.t)%type RR p_s p_t
       itr_s
       (LModTr.interp_stateE Any.t (iterV (LModTr.handle_callE prog_t) (tid_t, tp_t))
-        (Any.pair (ModTr.state_encode st_t) r_t)).
+        (st_t, r_t)).
   Proof using.
     intros Hin ? ?; eapply lookup_lt_Some in Hin as ?.
     giter_t; rewrite /= Hin; ss. gsteps_t. cSimpl.
-    rewrite ModTr.state_encode_decode //.
     giter_t; rewrite /= list_lookup_insert //=. gsteps_t. ired.
     rewrite list_insert_insert //.
   Qed.
@@ -337,20 +334,19 @@ Section props.
   Lemma gsim_SPut_src r g RR p_s p_t itr_t st_s prog_s tid_s tp_s key val k r_s :
     tp_s !! tid_s = Some (⇓cris (x <- trigger (SPut key val);; k x)) →
     map_Forall (const is_Some) st_s →
-    (gpaco7 _gsim (cpn7 _gsim) r g (Any.t * Any.t)%type (Any.t * Any.t)%type RR smj_top p_t
+    (gpaco7 _gsim (cpn7 _gsim) r g (lstateT * Any.t)%type (lstateT * Any.t)%type RR smj_top p_t
       (LModTr.interp_stateE Any.t
         (iterV (LModTr.handle_callE prog_s)
           (tid_s, <[tid_s := ⇓cris (k ())]> tp_s))
-        (Any.pair (ModTr.state_encode (<[key := Some val]> st_s)) r_s))
+        (<[key := Some val]> st_s, r_s))
       itr_t) →
-    gpaco7 _gsim (cpn7 _gsim) r g (Any.t * Any.t)%type (Any.t * Any.t)%type RR p_s p_t
+    gpaco7 _gsim (cpn7 _gsim) r g (lstateT * Any.t)%type (lstateT * Any.t)%type RR p_s p_t
       (LModTr.interp_stateE Any.t (iterV (LModTr.handle_callE prog_s) (tid_s, tp_s))
-        (Any.pair (ModTr.state_encode st_s) r_s))
+        (st_s, r_s))
       itr_t.
   Proof using.
     intros Hin ? ?; eapply lookup_lt_Some in Hin as ?.
     giter_s; rewrite /= Hin; ss. gsteps_s. cSimpl.
-    rewrite ModTr.state_encode_decode //.
     giter_s; rewrite /= list_lookup_insert //=. gsteps_s. ired.
     rewrite list_insert_insert //.
   Qed.
@@ -359,15 +355,15 @@ Section props.
     tp_s !! tid_s = Some (⇓cris (x <- trigger (Assume P);; k x)) →
     (∀ r_s2,
       ✓ r_s2 ∧ (Own r_s2 ⊢ |==> P ∗ Own r_s) →
-      gpaco7 _gsim (cpn7 _gsim) r g (Any.t * Any.t)%type (Any.t * Any.t)%type RR smj_top p_t
+      gpaco7 _gsim (cpn7 _gsim) r g (lstateT * Any.t)%type (lstateT * Any.t)%type RR smj_top p_t
         (LModTr.interp_stateE Any.t
           (iterV (LModTr.handle_callE prog_s)
             (tid_s, <[tid_s := ⇓cris (k ())]> tp_s))
-          (Any.pair st_s (r_s2↑)))
+          (st_s, r_s2↑))
         itr_t) →
-    gpaco7 _gsim (cpn7 _gsim) r g (Any.t * Any.t)%type (Any.t * Any.t)%type RR p_s p_t
+    gpaco7 _gsim (cpn7 _gsim) r g (lstateT * Any.t)%type (lstateT * Any.t)%type RR p_s p_t
       (LModTr.interp_stateE Any.t
-        (iterV (LModTr.handle_callE prog_s) (tid_s, tp_s)) (Any.pair st_s (r_s↑)))
+        (iterV (LModTr.handle_callE prog_s) (tid_s, tp_s)) (st_s, r_s↑))
       itr_t.
   Proof using.
     intros Hi Hk; pose proof Hi as Hlen; eapply lookup_lt_Some in Hlen.
@@ -388,17 +384,17 @@ Section props.
     tp_t !! tid_t = Some (⇓cris (x <- trigger (Assume P);; k x)) →
     (∃ r_t2,
       ✓ r_t2 ∧ (Own r_t2 ⊢ |==> P ∗ Own r_t) ∧
-      gpaco7 _gsim (cpn7 _gsim) r g (Any.t * Any.t)%type (Any.t * Any.t)%type RR p_s smj_top
+      gpaco7 _gsim (cpn7 _gsim) r g (lstateT * Any.t)%type (lstateT * Any.t)%type RR p_s smj_top
         (LModTr.interp_stateE Any.t (iterV (LModTr.handle_callE prog_s) (tid_s, tp_s)) st_s)
         (LModTr.interp_stateE Any.t
           (iterV (LModTr.handle_callE prog_t)
             (tid_t, <[tid_t := ⇓cris (k ())]> tp_t))
-          (Any.pair st_t (r_t2↑)))) →
-    gpaco7 _gsim (cpn7 _gsim) r g (Any.t * Any.t)%type (Any.t * Any.t)%type RR p_s p_t
+          (st_t, r_t2↑))) →
+    gpaco7 _gsim (cpn7 _gsim) r g (lstateT * Any.t)%type (lstateT * Any.t)%type RR p_s p_t
       (LModTr.interp_stateE Any.t
         (iterV (LModTr.handle_callE prog_s) (tid_s, tp_s)) st_s)
       (LModTr.interp_stateE Any.t
-        (iterV (LModTr.handle_callE prog_t) (tid_t, tp_t)) (Any.pair st_t (r_t↑))).
+        (iterV (LModTr.handle_callE prog_t) (tid_t, tp_t)) (st_t, r_t↑)).
   Proof using.
     intros Hin [r_t2 [Hr_t2 Hk]]; pose proof Hin as Hlen; eapply lookup_lt_Some in Hlen.
     giter_t; rewrite /= Hin /=. gstep_t. gsteps_t. cSimpl. ired. cSimpl. ired.
@@ -416,15 +412,15 @@ Section props.
     tp_s !! tid_s =
       Some (⇓cris (x <- trigger (AssumeRes r_s2);; k x)) →
     (✓ (r_s2 ⋅ r_s) →
-      gpaco7 _gsim (cpn7 _gsim) r g (Any.t * Any.t)%type (Any.t * Any.t)%type RR smj_top p_t
+      gpaco7 _gsim (cpn7 _gsim) r g (lstateT * Any.t)%type (lstateT * Any.t)%type RR smj_top p_t
         (LModTr.interp_stateE Any.t
           (iterV (LModTr.handle_callE prog_s)
             (tid_s, <[tid_s := ⇓cris (k ())]> tp_s))
-          (Any.pair st_s ((r_s2 ⋅ r_s)↑)))
+          (st_s, (r_s2 ⋅ r_s)↑))
         itr_t) →
-    gpaco7 _gsim (cpn7 _gsim) r g (Any.t * Any.t)%type (Any.t * Any.t)%type RR p_s p_t
+    gpaco7 _gsim (cpn7 _gsim) r g (lstateT * Any.t)%type (lstateT * Any.t)%type RR p_s p_t
       (LModTr.interp_stateE Any.t
-        (iterV (LModTr.handle_callE prog_s) (tid_s, tp_s)) (Any.pair st_s (r_s↑)))
+        (iterV (LModTr.handle_callE prog_s) (tid_s, tp_s)) (st_s, r_s↑))
       itr_t.
   Proof using.
     intros Hin Hk; pose proof Hin as Hlen; eapply lookup_lt_Some in Hlen.
@@ -441,16 +437,16 @@ Section props.
   Lemma gsim_AssumeRes_tgt r g RR p_s p_t st_t prog_s tid_t tp_t k r_t r_t2 itr_s :
     tp_t !! tid_t = Some (⇓cris (x <- trigger (AssumeRes r_t2);; k x)) →
     (✓ (r_t2 ⋅ r_t) ∧
-      gpaco7 _gsim (cpn7 _gsim) r g (Any.t * Any.t)%type (Any.t * Any.t)%type RR p_s smj_top
+      gpaco7 _gsim (cpn7 _gsim) r g (lstateT * Any.t)%type (lstateT * Any.t)%type RR p_s smj_top
         itr_s
         (LModTr.interp_stateE Any.t
           (iterV (LModTr.handle_callE prog_s)
             (tid_t, <[tid_t := ⇓cris (k ())]> tp_t))
-          (Any.pair st_t ((r_t2 ⋅ r_t)↑)))) →
-    gpaco7 _gsim (cpn7 _gsim) r g (Any.t * Any.t)%type (Any.t * Any.t)%type RR p_s p_t
+          (st_t, (r_t2 ⋅ r_t)↑))) →
+    gpaco7 _gsim (cpn7 _gsim) r g (lstateT * Any.t)%type (lstateT * Any.t)%type RR p_s p_t
       itr_s
       (LModTr.interp_stateE Any.t
-        (iterV (LModTr.handle_callE prog_s) (tid_t, tp_t)) (Any.pair st_t (r_t↑))).
+        (iterV (LModTr.handle_callE prog_s) (tid_t, tp_t)) (st_t, r_t↑)).
   Proof using.
     intros Hin [Hval Hk]; pose proof Hin as Hlen; eapply lookup_lt_Some in Hlen.
     giter_t; rewrite /= Hin /=. gstep_t; ss. gcNormT. cSimpl. ired. cSimpl. ired.
@@ -467,15 +463,15 @@ Section props.
     tp_s !! tid_s = Some (⇓cris (x <- trigger (Guarantee P);; k x)) →
     (∃ r_s2,
       ✓ r_s2 ∧ (Own r_s ⊢ |==> P ∗ Own r_s2) ∧
-      gpaco7 _gsim (cpn7 _gsim) r g (Any.t * Any.t)%type (Any.t * Any.t)%type RR smj_top p_t
+      gpaco7 _gsim (cpn7 _gsim) r g (lstateT * Any.t)%type (lstateT * Any.t)%type RR smj_top p_t
         (LModTr.interp_stateE Any.t
           (iterV (LModTr.handle_callE prog_s)
             (tid_s, <[tid_s := ⇓cris (k ())]> tp_s))
-          (Any.pair st_s (r_s2↑)))
+          (st_s, r_s2↑))
         itr_t) →
-    gpaco7 _gsim (cpn7 _gsim) r g (Any.t * Any.t)%type (Any.t * Any.t)%type RR p_s p_t
+    gpaco7 _gsim (cpn7 _gsim) r g (lstateT * Any.t)%type (lstateT * Any.t)%type RR p_s p_t
       (LModTr.interp_stateE Any.t
-        (iterV (LModTr.handle_callE prog_s) (tid_s, tp_s)) (Any.pair st_s (r_s↑)))
+        (iterV (LModTr.handle_callE prog_s) (tid_s, tp_s)) (st_s, r_s↑))
       itr_t.
   Proof using.
     intros Hi [r_s2 Hk]; pose proof Hi as Hlen; eapply lookup_lt_Some in Hlen.
@@ -496,16 +492,16 @@ Section props.
     tp_t !! tid_t = Some (⇓cris (x <- trigger (Guarantee P);; k x)) →
     (∀ r_t2,
       ✓ r_t2 ∧ (Own r_t ⊢ |==> P ∗ Own r_t2) →
-      gpaco7 _gsim (cpn7 _gsim) r g (Any.t * Any.t)%type (Any.t * Any.t)%type RR p_s smj_top
+      gpaco7 _gsim (cpn7 _gsim) r g (lstateT * Any.t)%type (lstateT * Any.t)%type RR p_s smj_top
         itr_s
         (LModTr.interp_stateE Any.t
           (iterV (LModTr.handle_callE prog_t)
             (tid_t, <[tid_t := ⇓cris (k ())]> tp_t))
-          (Any.pair st_t (r_t2↑)))) →
-    gpaco7 _gsim (cpn7 _gsim) r g (Any.t * Any.t)%type (Any.t * Any.t)%type RR p_s p_t
+          (st_t, r_t2↑))) →
+    gpaco7 _gsim (cpn7 _gsim) r g (lstateT * Any.t)%type (lstateT * Any.t)%type RR p_s p_t
       itr_s
       (LModTr.interp_stateE Any.t
-        (iterV (LModTr.handle_callE prog_t) (tid_t, tp_t)) (Any.pair st_t (r_t↑))).
+        (iterV (LModTr.handle_callE prog_t) (tid_t, tp_t)) (st_t, r_t↑)).
   Proof using.
     intros Hin ?; pose proof Hin as Hlen; eapply lookup_lt_Some in Hlen.
     giter_t; rewrite /= Hin /=. gstep_t. gsteps_t. cSimpl. ired. cSimpl. ired.
